\documentclass{article}
\usepackage{amsmath, amssymb, bm}

\begin{document}

\begin{center}
    {\fontsize{25}{16}\selectfont \textbf{AP Calculus AB Formulas:}} % Adjusted font size and bold text
\end{center}

\section*{\textbf{Derivatives:}}

\textbf{Point-Slope Form:}
\[
y - y_1 = m(x - x_1)
\]

\textbf{Limit Definition of Derivative:}
\[
\frac{d}{dx} f(x) = \lim_{h\rightarrow 0} \frac{f(x+h) - f(x)}{h}
\]

\[
\frac{d}{dx} f(x) = \lim_{x\rightarrow c} \frac{f(x) - f(c)}{x-c}
\]

\textbf{Power Rule:}
\[
\frac{d}{dx} x^n = n x^{n - 1}
\]

\textbf{Constant Rule:}
\[
\frac{d}{dx} c = 0
\]

\textbf{Product Rule:}
\[
\frac{d}{dx} \left( f(x) \cdot g(x) \right) = f'(x) g(x) + f(x) g'(x)
\]

\textbf{Quotient Rule:}
\[
\frac{d}{dx} \left( \frac{f(x)}{g(x)} \right) = \frac{f'(x) g(x) - f(x) g'(x)}{(g(x))^2}
\]

\textbf{General Power Rule (u-substitution):}
\[
\frac{d}{dx} u^n = n u^{n - 1} u'
\]

\textbf{Chain Rule:}
\[
\frac{d}{dx} f(g(x)) = f'(g(x)) g'(x)
\]

\textbf{Implicit Differentiation:} Factor out \( y' \).

\textbf{Increasing Function:}
\[
f'(x) \geq 0
\]

\textbf{Decreasing Function:}
\[
f'(x) \leq 0
\]

\textbf{Concave Up:}
\[
f''(x) \geq 0
\]

\textbf{Concave Down:}
\[
f''(x) \leq 0
\]

\section*{\textbf{Mean Value Theorem (MVT) and Integrals:}}

\textbf{Mean Value Theorem (MVT):}
\[
f'(c) = \frac{f(b) - f(a)}{b - a}
\]

\textbf{Reverse Power Rule:}
\[
\int x^n \, dx = \frac{x^{n+1}}{n+1} + C, \quad n \neq -1
\]

\textbf{Reverse Constant Rule:}
\[
\int k \, dx = kx + C
\]

\textbf{Reverse Chain Rule:}
\[
\int u^n u' \, dx = \frac{u^{n+1}}{n+1} + C, \quad n \neq -1
\]

\textbf{Area Under the Curve:}
\[
\int_{a}^{b} f(x) \, dx = F(b) - F(a) \text{, Where } F(x) \text{ is the antiderivative of } f(x)
\]

\textbf{Fundamental Theorem of Calculus:}
\[
\int_{a}^{b} f'(x) \, dx = f(b) - f(a)
\]

\textbf{Start + Accumulation:}
\[
f(b) = f(a) + \int_{a}^{b} f'(x) \, dx
\]

\textbf{Derivative of an Integral:}
\[
\frac{d}{dx} \int (2x-3)\, dx = 2x-3
\]

\textbf{Second Fundamental Theorem:}
\[
\frac{d}{dx} \int_{a}^{x} f(t) \, dt = f(x)
\]

\section*{\textbf{Exponential and Logarithmic Functions:}}

\textbf{Derivative of Exponential Function:}
\[
\frac{d}{dx} e^x = e^x
\]

\textbf{Derivative of General Exponential Function:}
\[
\frac{d}{dx} a^x = a^x \ln a
\]

\textbf{Derivative of Natural Log:}
\[
\frac{d}{dx} \ln x = \frac{1}{x}
\]

\textbf{Derivative of Logarithm (Base a):}
\[
\frac{d}{dx} \log_a x = \frac{1}{x \ln a}
\]

\textbf{Integral of Exponential Function:}
\[
\int e^x \, dx = e^x + C
\]

\textbf{Integral of General Exponential Function:}
\[
\int a^x \, dx = \frac{a^x}{\ln a} + C
\]

\textbf{Integral of Natural Log:}
\[
\int \ln x \, dx = x \ln x - x + C
\]

\textbf{Integral of Exponential Function (Reverse Chain Rule):}
\[
\int e^{u} u' \, dx = e^{u} + C
\]

\textbf{Integral of General Exponential Function (Reverse Chain Rule):}
\[
\int a^{u} u' \, dx = \frac{a^{u}}{\ln a} + C
\]

\textbf{Integral of Natural Log (Reverse Chain Rule):}
\[
\int \ln u \, du = u \ln u - u + C
\]

\section*{\textbf{Trigonometric Functions:}}

\textbf{Derivative of Sine Function:}
\[
\frac{d}{dx} \sin x = \cos x
\]

\textbf{Derivative of Cosine Function:}
\[
\frac{d}{dx} \cos x = -\sin x
\]

\textbf{Derivative of Tangent Function:}
\[
\frac{d}{dx} \tan x = \sec^2 x
\]

\textbf{Derivative of Cosecant Function:}
\[
\frac{d}{dx} \csc x = -\csc x \cot x
\]

\textbf{Derivative of Secant Function:}
\[
\frac{d}{dx} \sec x = \sec x \tan x
\]

\textbf{Derivative of Cotangent Function:}
\[
\frac{d}{dx} \cot x = -\csc^2 x
\]

\textbf{Integral of Sine Function:}
\[
\int \sin x \, dx = -\cos x + C
\]

\textbf{Integral of Cosine Function:}
\[
\int \cos x \, dx = \sin x + C
\]

\textbf{Integral of Tangent Function:}
\[
\int \tan x \, dx = -\ln|\cos x| + C
\]

\textbf{Integral of Cosecant Function:}
\[
\int \csc x \, dx = -\ln|\csc x + \cot x| + C
\]

\textbf{Integral of Secant Function:}
\[
\int \sec x \, dx = \ln|\sec x + \tan x| + C
\]

\textbf{Integral of Cotangent Function:}
\[
\int \cot x \, dx = \ln|\sin x| + C
\]

\end{document}